wip: barrier state machines

src/lib/kuiper/Kuiper.Barrier.fsti
@@ -2,27 +2,28 @@ module Kuiper.Barrier
 
 #lang-pulse
 
-open Kuiper.Common
-open Pulse.Lib.Pervasives
-open Kuiper.ForEvery
 open FStar.Tactics.V2
 open Kuiper.Base
+open Kuiper.Common
+open Kuiper.ForEvery
 open Kuiper.SizeT
+open Kuiper.StateMachine
+open Pulse.Lib.Pervasives
 
 (* A barrier over nthreads. This is for specification only,
 there is no runtime representation for it, nor a handle-like
 type, as this models the builtin CUDA __syncthreads() function. *)
 
-type barrier_side (n:nat) =
-  it : nat ->
+type barrier_side (stm : stm_t) (n:nat) =
+  s : stm.state0 ->
   tid : natlt n ->
   slprop
 
-type barrier_transform (#n:nat) (p q : barrier_side n) =
-  it:nat ->
+type barrier_transform (#n:nat) (#stm:stm_t) (p q : barrier_side stm n) =
+  s : stm.state0 ->
   stt_ghost unit emp_inames
-           (requires forall+ (i:natlt n). p it i)
-           (ensures  fun _ -> forall+ (i:natlt n). q it i)
+           (requires forall+ (i:natlt n). p s i)
+           (ensures  fun _ -> forall+ (i:natlt n). q s i)
 
 (* A token representing that there is a barrier in scope.
    This is a ghost token, and is not used at runtime. *)
@@ -30,20 +31,22 @@ type barrier_transform (#n:nat) (p q : barrier_side n) =
 (* A token representing that there is a barrier in scope with contract (p,q).
 This does not change as we wait on the barrier. *)
 [@@no_mkeys]
-val barrier_tok (#n:nat) (p q : barrier_side n) : slprop
+val barrier_tok (#n:nat) (#stm : stm_t) (p q : barrier_side stm n) : slprop
 
 (* A token that we are at iteration `it` of the current barrier. *)
 [@@no_mkeys]
-val barrier_state (it : nat) : slprop
+val barrier_state (#stm:stm_t) (s : st stm.state0) : slprop
 
 instance val barrier_tok_sendable
   (n:nat)
-  (p q : barrier_side n)
-: is_send_across block_of (barrier_tok #n p q)
+  (stm : stm_t)
+  (p q : barrier_side stm n)
+  : is_send_across block_of (barrier_tok #n #stm p q)
 
 instance val barrier_state_sendable
-  (it : nat)
-: is_send_across block_of (barrier_state it)
+  (#stm:stm_t)
+  (s : st stm.state0)
+  : is_send_across block_of (barrier_state s)
 
 (* Creating a barrier for n threads. Note how this is a
    ghost function!. The 'pf' argument is a proof, once and
@@ -53,22 +56,24 @@ instance val barrier_state_sendable
 ghost
 fn mk_barrier
   (n: nat)
-  (p q : barrier_side n)
+  (#stm : stm_t)
+  (p q : barrier_side stm n)
   (pf : barrier_transform p q)
   requires can_create_barrier n
   ensures  consumed_can_create_barrier
-  ensures  forall+ (i:natlt n). barrier_tok p q ** barrier_state 0
+  ensures  forall+ (i:natlt n). barrier_tok p q ** barrier_state (S stm.init)
 
 (* Wait on the barrier. This function blocks until all threads call it
    simultaneously. Each thread provides the current p
    and gets the current q. The iteration counter is incremented. *)
 fn barrier_wait
-  ()
+  (#stm : stm_t)
   (#n : erased nat)
-  (#p #q : barrier_side n)
-  (#it : erased nat)
+  ()
+  (#p #q : barrier_side stm n)
+  (#it : erased stm.state0)
   (#tid : enatlt n)
   preserves barrier_tok p q
   preserves thread_id n tid
-  requires barrier_state it     ** p it tid
-  ensures  barrier_state (it+1) ** q it tid
+  requires barrier_state (S it)        ** p it tid
+  ensures  barrier_state (stm.next it) ** q it tid
