src/lib/kuiper/Kuiper.StateMachine.fst
@@ -1,0 +1,77 @@
+module Kuiper.StateMachine
+
+open Kuiper.Common
+
+type st (st0:Type0) = 
+  | S of st0
+  | Done
+
+noeq
+type stm_t = {
+  state0 : Type0;
+  init  : state0;
+  next  : state0 -> st state0;
+}
+
+// N steps
+let fin_n (n:pos) : stm_t = {
+  state0 = natlt n;
+  init = 0;
+  next = (fun s -> if s = n-1 then Done else S (s + 1));
+}
+
+let seq (stm1 stm2 : stm_t) : stm_t = {
+  state0 = either stm1.state0 stm2.state0;
+  init = Inl (stm1.init);
+  next = (fun s ->
+    match s with
+    | Inl s1 -> (
+      match stm1.next s1 with
+      | S s1' -> S (Inl s1')
+      | Done  -> S (Inr stm2.init)
+    )
+    | Inr s2 -> (
+      match stm2.next s2 with
+      | S s2' -> S (Inr s2')
+      | Done  -> Done)
+  );
+}
+
+let repeat (n:pos) (stm0 : stm_t) : stm_t = {
+  state0 = (natlt n & stm0.state0);
+  init = (0, stm0.init);
+  next = (fun s ->
+    let (i, s0) = s in
+    match stm0.next s0 with
+    | S s0' -> S (i, s0')
+    | Done  -> 
+      if i = n - 1 then Done
+      else S (i + 1, stm0.init)
+  );
+}
+
+type even_odd_t = | Even | Odd
+
+// Infinite
+let even_odd_inf : stm_t = {
+  state0 = even_odd_t;
+  init = Even;
+  next = (fun s ->
+    match s with
+    | Even -> S Odd
+    | Odd  -> S Even);
+}
+
+// Just two
+let even_odd : stm_t = {
+  state0 = even_odd_t;
+  init = Even;
+  next = (fun s ->
+    match s with
+    | Even -> S Odd
+    | Odd  -> Done);
+}
+
+// Usual stm_t for barrier in GEMMs
+let even_odd_n (n:pos) : stm_t =
+  repeat n even_odd
